Content-Type: text/enriched
Text-Width: 80

Limits -*- mode: org -*-


<x-color><param>#FD971F</param>* Infimum and Supremum of sequences

</x-color><x-color><param>#A6E22E</param>|Let $(x_n)$ be a monotonic sequence.</x-color>  
<x-color><param>#A6E22E</param>|If $(x_n)$ is bounded then it is convergent</x-color>
<x-color><param>#A6E22E</param>|and $\lim_{n\to\infty} x_n = \sup(x_n, n \in \mathbb{N})$ or $\inf(x_n, n \in \mathbb{N})$</x-color>
<x-color><param>#75715E</param>:proof:</x-color>

Let $(x_n)$ be increasing and bounded and $x = \sup(x_n, n \in \mathbb{N})$


Let $\varepsilon > 0$
then $x - \varepsilon$ is not upper bound.


You can find $N$ s.t. $x - \varepsilon << x_n \leq x$
Since $(x_n)$ increasing
$x \geq x_N$


Let $(-x_n)$ be increasing and bounded
So $\lim_{n\to\infty} (-x_n) = \sup(-x_n) = -\inf(x_n)$
So $\lim_{n\to\infty} = \inf(x_n)$

<x-color><param>#75715E</param>:END:</x-color>

<x-color><param>#75715E</param>:examples:</x-color>

1. $x_n = \frac{1}{n}$

   $x_n$ is decreasing and bounded, so it converges to $\inf(\frac{1}{n}) = 0$


2. $x_n = 1 + \frac{1}{2} + ... + \frac{1}{n}$

   $(x_n)$ is increasing. We will show it is not bounded.

   $x_n = 1 + \frac{1}{2} + (\frac{1}{3} + \frac{1}{4}) + ... \\

   \geq 1 + \frac{1}{2} + (\frac{1}{4} + \frac{1}{4}) + ... = 1 + \frac{n}{2}$

   So $x_n$ is not bounded


3. Let $x_n$ be defined

   $x_1 = 1$

   $x_{n+1} = \frac{1}{4}(2x + 3)$

   First prove that $x_n$ is increasing. (by induction)

   $x_1 << x_2$

   $\frac{1}{4}(2x_n + 3) \leq \frac{1}{4}(2x_{n+1} + 3)$

   so $x_n \leq x_{n+1}$

   <bold>*Show bounded*</bold> (by induction)

   $x_1 \leq 2$

   Assume $x_n \leq 2$, then

   $x_{n+1} = \frac{1}{4}(2x_n + 3) \leq \frac{7}{4} \leq 2$

   so $x_n$ is bounded.

   Now to find the limit. $x_n = x_{n+1}$

   so $x = \frac{1}{4}(2x + 3) \Rightarrow x = \frac{3}{2}$

<x-color><param>#75715E</param>:END:</x-color>


<x-color><param>#FD971F</param>* Subsequences and Bolzana-Weierstrauss

</x-color>*subsequence*
<x-color><param>#A6E22E</param>|Let $(y_n)$ be a sequence.</x-color>
<x-color><param>#A6E22E</param>|If the sequence $(x_n) \subseteq (y_n)$</x-color>

<x-color><param>#A6E22E</param>|Then $(x_n)$ is a subsequence of $(y_n)$</x-color>
<x-color><param>#75715E</param>:examples:</x-color>

 $(2,4,6,8,...)$ subsequence of $(1,2,3,4,...)$
 


 $x_n = (-1)^n$     $(-1,1,-1,1,...)$
 $x_n = 1$        $(1,1,1,1,...)$
 $x_n = -1$       $(-1,-1,-1,-1,...)$  

<x-color><param>#75715E</param> :END:</x-color>


<x-color><param>#A6E22E</param>|Let $(x_n)$ be a convergent sequence</x-color>
<x-color><param>#A6E22E</param>|Then all subsequences are also convergent and the limits are the same.</x-color>

<x-color><param>#75715E</param>:proof:</x-color>

Let $x = \lim_{x\to \infty} x_n$
Let $\varepsilon > 0$.  We can find $f(\varepsilon)$ s.t. $|x_n - x| \leq \varepsilon$ for $n \geq f(\varepsilon)$
Since $n_k$ is strictly increasing, $n_k \geq k$
For $k \geq f(\varepsilon), n_k \geq k \geq f(\varepsilon)$
so $|x_{n_k} - x| \leq \varepsilon$ and $\lim_{k\to\infty} x_{n_k} = x$

<x-color><param>#75715E</param>:END:</x-color>

<x-color><param>#75715E</param>:examples:</x-color>

$x_n = \frac{1}{n^4}$
Since $$n^4 \in \mathbb{N}$$, $x_n$ is a subsequence of $\frac{1}{n}$.
So $x_n$ must also converge to 0.


$x_n = (-1)^n$
$x_{2n} = 1, \lim_{n\to\infty} = 1$
$x_{2n+1} = 1, \lim_{n\to\infty} = -1$
So $x_n$ is divergent

<x-color><param>#75715E</param>:END:</x-color>


Let $(x_n)$ be a sequence.  Then
$(x_n)$ does not converge
