
:examples:
1. x_n = n
   Let $M \geq 0 for n\geqM, x_n \geq M$
   So $(x_n)$ goes to infinity
1. $x_n = 1 - \frac{1}{n} + n \geq M$
2. $x_n = n^2 - n = n(n-1) \geq (n-1)^2$

|Let $(x_n) be increasing and not bounded.  Then $\lim_{n \Rightarrow \infty} x_n = \infty
|Let $(x_n) be decreasing and not bounded.  Then $\lim_{n \Rightarrow -\infty} x_n = -\infty
:proof:
Let $(x_n)$ be increasing and not bounded
Let $M \geq 0$, Since $(x_n)$ is not bounded, you can find $n \geq 0$ s.t. $x_n \geq M$
For $k \geq n, x_k \geq x_n$ so $x_k \geq x_n \geq M$

If $(x_n)$ is decreasing and bounded, $(-x_n)$ is increasing and not bounded
so $\lim_{n \Rightarrow \infty} -x_n = \infty$
$\lim_{n \Rightarrow \infty} x_n = -\infty$
:END:

Let $(x_n),(y_n)$ be sequences s.t. $(x_n) \geq (y_n)$
$\lim_{n \Rightarrow \infty} (y_n) = \infty$ implies $\lim_{n \Rightarrow \infty} (y_n) = \infty$
