#+TITLE: ECE382 - Control Systems - Spring 2016
* Poles and Zeros
** Open loop

** Closed loop

#+attr_html: width 400
[[./loop.png]]

$T(s) = \frac{C(s)}{R(s)} = \frac{G(s)}{1 + G(s)H(s)}$

roots of $G(s)$: closed loop zeros

roots of $1 + G(s)$: closed loop poles

$\frac{B}{E} = G(s)H(s)$

roots of $G(s)H(s)$: zeros

poles of $G(s)H(s)$: poles

* Characteristic Equation

#+begin_definition
Characteristic equation - $1 + G(s)H(s) = 1 + \frac{N_1N_2}{D_1D_2} = \frac{D_1D_2 + N_1N_2}{D_1D_2}$
#+end_definition

$D_1D_2 + N_1N_2$: closed-loop poles

$D_1D_2$: open-loop poles

transfer functions need to be in polynomial form
#+begin_examples
1. $G_2(s) = \frac{1}{s-1}$

   $s = +1 \Rightarrow e^t$, so system is unstable
#+end_examples

* Second-order systems
** Characterization
*second-order transfer function* - \[T(s) = \frac{N}{N + D} = \frac{w_n^2}{s^2 + 2\zeta w_ns + w_n^2}\]

$\zeta = \cos (\theta)$: damping coefficient

$w_n$: undamped natural frequency

$w_d = w_n \sqrt{1 - \zeta^2}$ - damped frequency

$\zeta \omega_n$: attenuation

use quadratic formula to find poles

\begin{equation*}
s_1,s_2 =
  \begin{cases}
    -\zeta w_n +- w_n \sqrt{\zeta^2 -1} & \zeta \geq 0 \\ 
    -\zeta w_n +- w_n \sqrt{1 - \zeta^2} & 0 < \zeta < 1
  \end{cases}
\end{equation*}


[[./damping.png]]

Four cases:
1. $\zeta = 0$: infinite signal
2. $\zeta = 1$: critically-damped$
3. $0 < \zeta < 1$ - infinite oscillations
4. $\zeta > 1$ - overdamped 

** Analysis
[[./performance.png]]


*** Overshoot
$M_P = e^{\dfrac{-\pi \zeta}{\sqrt{1 - \zeta^2}}}$ - percent overshoot

#+begin_derivation
\begin{align*}
M_P & = \frac{c(t_p) - c(\infty)}{c(\infty)} \\
    & = c(t_p) \\
    & = e^{\dfrac{-\pi \zeta}{\sqrt{1 - \zeta^2}}}
\end{align*}
#+end_derivation

$t_p = \frac{\pi}{\omega_d}$ - time to first overshoot
*** Rise Time
$t_r$ - rise time ( to 100% of target value )

#+begin_derivation
\begin{eqnarray*}
\frac{d}{dt}[c(t)] = 0 \\ 
\Rightarrow t_p = \frac{\pi}{w_d}
\end{eqnarray*}
#+end_derivation

*** Settling Time
$t_s = \frac{4}{\zeta \omega_n}$ - settling time
#+begin_derivation
\begin{align*}
e^{-\zeta \omega_n t} = .02 \\
\Rightarrow t & = \frac{-\ln(.02)}{\zeta \omega_n} \\
t & \approx \frac{4}{\zeta \omega_n}
\end{align*}
#+end_derivation

Damped sinusoid with unit step input
$c(t) = 1 - \beta e^{-\zeta \omega_n t} \sin(\omega_d t + \theta)$

#+begin_examples
1. [[./loop2.png]]

   $G(s) = \frac{k}{s(s+p)}$

2. [[./loop3.png]]

   $T(s) = \frac{G}{1+G} = \frac{N}{N + D} = \frac{k}{s^2 + ps + k}$

   Find K and P s.t.t $R(s) = \frac{1}{s}, t_s = 2, M_P = .1$

   In canonical form, $k = {\omega_n}^2, p = 2 \zeta \omega_n$

   $M_P = .1 = e^{\dfrac{-\pi \zeta}{\sqrt{1 - \zeta^2}}}$
#+end_examples
 
*** Steady State Error
$E(s) = \frac{R(S)}{1+G(S)H(S)}$

We will only study the error when $R(S)$ is a step, ramp, or exponential function

Let $r(t) = ku(t),R(s) = \frac{k}{s}$

$E(s) = \dfrac{\dfrac{k}{s}}{1 + G(s)H(s)}$

**** Finite value theorem
Requirements
1. Poles of $F(t)$ must have negative real parts to be stable
2. $F(s)$ has at most 1 pole at the origin

$f_{ss} = f(\infty) = \lim_{t \rightarrow \infty} f(t) = lim_{s \rightarrow 0} s F(s)$


_steady state error_
#+begin_definition
$e_{ss} = \frac{k}{1 + \lim_{s \rightarrow 0} k_p}$
#+end_definition
#+begin_derivation
\begin{align*}
e_{ss} & = \lim_{s \rightarrow 0} s E(s) \\
& = \lim_{s \rightarrow 0} \frac{k}{1 + G(s)H(s)} \\
& = \frac{k}{1 + \lim_{s \rightarrow 0} G(s)H(s)} \\
& = \frac{k}{1 + \lim_{s \rightarrow 0} k_p}
\end{align*}
#+end_derivation

_static error constant_ (error contribution from a step input)
#+begin_definition
$k_p = \lim_{s \rightarrow 0} G(s)H(s) = \frac{K(s+Z_1)...(s+Z_n)}{s^N(s+P_1)...(s+P_n)}$ 
#+end_definition

_static velocity constant_ (error contribution from a ramp input)
#+begin_definition
$k_v = \lim_{s \rightarrow 0} sG(s)H(s) = \frac{sK(s+Z_1)...(s+Z_n)}{s^N(s+P_1)...(s+P_n)}$ 
#+end_definition

_static acceleration constant_ (error contribution from a parabolic input)
#+begin_definition
$k_v = \lim_{s \rightarrow 0} s^2G(s)H(s) = \frac{s^2K(s+Z_1)...(s+Z_n)}{s^N(s+P_1)...(s+P_n)}$ 
#+end_definition

So if the input is $r(t) = (A t r(t) + B r(t) + C) u(t)$

$e_{ss} = \frac{A}{k_a} + \frac{B}{k_v} + \frac{c}{1 + k_p}$

#+begin_examples
1. Consider unity feedback

   $G(s) = \frac{k}{s(s+1)(s+2)}$

   Find the steady state error

   $R(s) = \frac{3}{s} + \frac{2}{s^2}$

   $k_p = lim_{s \to 0} G(s) = \infty$

   $k_v = lim_{s \to 0} s G(s) = \frac{1}{k}$

   $e_{ss} = \frac{3}{1 + k_p} + \frac{2}{k_v} = \frac{3}{1 + \infty} + \frac{2}{\frac{k}{2}} = \frac{4}{k}$

   So as $k \to \infty$, $e_{ss} = 0$
#+end_examples
*You must also prove the stability of the system to prove that $e_{ss}$ exists*

*** Stability
#+begin_definition
_bibo_ - bounded input bounded output
#+end_definition
#+begin_examples
1. Unity feedback with $G(s) = \frac{2}{s(s+3)}$

   $T(s) = \frac{C(s)}{R(s)} = \frac{2}{(s+1)(s+3)}$

   If the input is step, $R(s) = \frac{1}{s}$

   So $C(s) = \frac{2}{s(s+1)(s+3)} = \frac{A}{s} + \frac{B}{s+1} + \frac{C}{s+2}$
   
   \begin{align*}
   Q(s) & = 1 + G(s) = 0 \\
   & = \frac{s(s+1)(s+2) + k}{s(s+1)(s+2)} = 0
   \end{align*}

   Since the closed-loop poles (num of char eqn) are in LHP, system is stable.
   
#+end_examples

Assume feedback system with $G(s)$ and $H(s)$

$Q(s) = 1 + G(s)H(s) = \frac{D_1D_2 + N_1N_2}{D_1D_2} = 0$

$D_1D_2 + N_1N_2$ - closed-loop poles

Three ways to solve for stability
1. Matlab
2. Routh-Hurwitz Stability Test
3. Root locus

*** Routh-Hurwitz Stability Test
1. Construct first two rows
2. Construct next rows based on first two
3. Count number of sign changes in first column to find RHP poles

Let $Q(s) = a_ns^n + a_{n-1}s^{n-1} + ... + a_1s + a_0 = 0$

If $n$ is even

| $s^n$     | $a_n$     | $a_{n-2}$ | ... | $a_0$ |
| $s^{n-1}$ | $a_{n-1}$ | $a_{n-3}$ | ... | $a_1$ |

If $n$ is odd

| $s^n$     | $a_n$     | $a_{n-2}$ | ... | $a_0$ |
| $s^{n-1}$ | $a_{n-1}$ | $a_{n-3}$ | ... | $a_1$ |

Construct rest of table

| $s^{n-2}$   | $b_1$ | $b_2$ | ... | $b_{n+1}$ |
| $s^{n-3}$ | $c_1$ | $c_2$ | ... | $c_{n+1}$ |
| $s^{n-4}$ | $d_1$ | $d_2$ | ... | $d_{n+1}$ |

Where 
\begin{align*}
b_1 & = \frac{a_{n_1}a_{n-2} - a_na_{n-3}}{a_{n-1}} \\
b_2 & = \frac{a_{n_1}a_{n-2} - a_na_{n-4}}{a_{n-2}} \\
...
\end{align*}

If $b_n$ is zero, use $\varepsilon$ as a placeholder for a positive number.
Assume blank entries to be 0.

If a row is zero, differentiate the row above it and replace the zeros with the coefficients.

The number of sign changes in the first column is equal to
the number of poles in RHP.

If the last and third to last row have the same sign,
then the poles are on the imaginary axis.

#+begin_examples
1. Let $Q(s) = s(s+1)(s+2) + 3 = s^3 + 3s^2 + 2s + 7 = 0$
   | $s^3$ |               1 |   2 |
   | $s^2$ |               3 |   7 |
   | $s$   | $\frac{-1}{3}$  | nan |
   | $s^0$ |               7 | nan |
   
   Two sign changes means two RHP poles, 1 LHP pole, so the system is unstable.

2. Let $Q(s) = s^3 + 4s^2 + s - 6$
   | $s^3$ |              1 |  1 |
   | $s^2$ |              4 | -6 |
   | $s^1$ | $\frac{10}{4}$ |    |
   | $s^0$ |             -6 |    |

    One sign change means one RHP pole, 2 LHP poles, so the system is unstable.

3. Let $Q(s) = s^3 - s^2 - s + 1 = 0$
   | $s^3$ |             1 | -1 |
   | $s^2$ |            -1 |  1 |
   | $s^1$ | $\varepsilon$ |    |
   | $s^0$ |             1 |    |
#+end_examples

#+begin_examples
1. $G(s) = \frac{k}{s(s+1)(s+2)}$
   $k_p = \lim_{s \to 0} G(s) = \infty$
   $k_v = \lim_{s \to 0} s G(s) = \frac{k}{2}$
   $e_{ss} = \frac{3}{1 + k_p} + \frac{2}{k_v} = \frac{4}{k}$
   $Q(s) = s(s+1)(s+2) + K = s^3 + 3s^2 + 2s + K$
   | $s^3$ | $1$             | $2$ |
   | $s^2$ | $3$             | $K$ |
   | $s^1$ | $\frac{6-K}{3}$ |     |
   | $s^0$ | $0$             |     |
2. $T(s) = \frac{G}{1+G} = \frac{k}{s^2 +2s + K}$

   $Q(s) = \frac{s^2 + 2s + K}{s(s+2)}$

   $Q(s) = s^2 + 2s + K$

   | $s^2$ | 1    | K |
   | $s^1$ | $2$  |   |
   | $s^0$ | $2K$ |   |
   
   System is stable for all $K > 0$

   $s_1,s_2 = \frac{-2 +- \sqrt{4 - 4K}}{2} = -1 += \sqrt{1-K}$

   Let $K=0$, then $s_1,s_2 = 0, -2$

   Let $K=.5$, then $s_1,s_2 = -0.29, -1.707$

   Overdamped

   Let $K=1$, then $s_1,s_2 = -1, 1$

   Critically damped

   Let $K=2$, then $s_1,s_2 = -1+j, 1+j$

   Underdamped
   
   [[./root_locus.png]]
#+end_examples
*** Root Locus
#+begin_examples
\begin{align*}
Q(s) = 1 + G(s)H(s) & = 1 + \frac{K \sum_{i=1}^{N_z} (s + Z_i)}{\sum_{j=1}^{N_p} (s + P_j)} \\
& = 1 + \frac{K \sum_{i=1}^{N_z} (s + Z_i)}{\sum_{j=1}^{N_p} (s + P_j)}
\end{align*}

$KG(s)H(s) = -1 + j0$

$|KG(s)H(s)| = 1$

$$\angle KG(s)H(s) = \pi(1 + 2m), m=0,1,2,...$$
#+end_examples
